\subsection{Reformulation of the BÃ¼rmann-Lagrange series}

\begin{align}
        g(z) &= a + \sum_{n \geq 1} \frac{(z-f(a))^n}{n!}
        \lim_{\omega \to a}\frac{d^{n-1}}{d\omega^{n-1}}
        \left[ \left(\frac{\omega - a}{f(\omega) - f(a)} \right)^n\right] 
\end{align}

let substitute the limit

\begin{align}
        \Psi(a) &= \lim_{\omega \to a}\left[ (\omega-a)^n(f(\omega)
        - f(a))^{-n}\right] \\
        &= \lim_{\omega \to a}\sum_{k=0}^{n-1}\binom{n-1}{k}(\omega 
        - a)^{k-1}(k)_{n-k-1}\left( (f(\omega) - f(a))^{-n}\right)^{(k)}\\
\end{align}

and

\begin{align}
        \Lambda(k, a)& = \left( (f(\omega) - f(a))^{-n}\right)^{(k)} \\
        &= \sum_{\lambda = 0}^{\infty}\binom{-n}{\lambda}f(a)^\lambda
        f(\omega)^{-n-k} \\
\end{align}
hence

\begin{align}
        \Psi(a) &= \lim_{\omega \to a}\sum_{k=0}^{n-1}\binom{n-1}{k}(\omega
        - a)^{k-1}(k)_{n-k-1}\left( (f(\omega) - f(a))^{-n}\right)^{(k)}\\
        &= \lim_{\omega \to a}\sum_{k=0}^{n-1}\binom{n-1}{k}(\omega -
        a)^{k-1}(k)_{n-k-1}\sum_{\lambda = 0}^{\infty}\binom{-n}{
        \lambda}f(a)^\lambda \left(f(\omega)^{-n-k}\right)^{(k)} \\
        &= \sum_{k=0}^{n-1}\binom{n-1}{k}(k)_{n-k-1}\lim_{\omega 
        \to a}(\omega -a)^{k-1}\sum_{\lambda = 0}^\infty \binom{-n
        }{\lambda}\left( f(\omega)^{-n-\lambda}\right)^{(k)} \\
        &= \sum_{k=0}^{n-1}\binom{n-1}{k}(k)_{n-k-1} \sum_{\lambda 
        = 0}^{\infty}\binom{-n}{\lambda} \lim_{\omega \to a}\left[
        \frac{(f(\omega)^{-n-\lambda})^{(k)}}{(\omega - a)^{1-k}}\right]
\end{align}

so we get the expression

\begin{align}
        g(z) = a+ \sum_{n=1}^{\infty} \frac{(z-f(a))^n}{n!}\sum_{k=0}^{n-1}
        \binom{n-1}{k}(k)_{n-k-1}\sum_{\lambda=0}^\infty \binom{-n}{\lambda}
        \lim_{\omega \to a}\left[ \frac{(f(\omega)^{-n-\lambda})^{(k)}}{(\omega - a)^{1-k}}\right]
\end{align}
